refactor and done

Foundation/Modal/Neighborhood/Logic/E4.lean
@@ -1,6 +1,12 @@
-import Foundation.Modal.Neighborhood.Hilbert
+import Foundation.Modal.Neighborhood.AxiomC
 import Foundation.Modal.Neighborhood.AxiomGeach
+import Foundation.Modal.Neighborhood.AxiomM
+import Foundation.Modal.Neighborhood.AxiomN
 import Foundation.Modal.Neighborhood.Logic.E
+
+@[simp]
+lemma Set.inter_eq_univ {s t : Set α} : s ∩ t = Set.univ ↔ s = Set.univ ∧ t = Set.univ := by
+  simpa using @Set.sInter_eq_univ _ {s, t};
 
 namespace LO.Modal
 
@@ -16,6 +22,47 @@ instance : Frame.simple_blackhole.IsTransitive := by
 
 @[reducible] protected alias Frame.IsE4 := Frame.IsTransitive
 protected abbrev FrameClass.E4 : FrameClass := { F | F.IsE4 }
+
+
+section
+
+abbrev Frame.trivial_nontransitive : Frame := ⟨
+  Fin 2,
+  λ w =>
+    match w with
+    | 0 => ∅
+    | 1 => {Set.univ}
+⟩
+
+instance : Frame.trivial_nontransitive.IsRegular := by
+  constructor;
+  rintro X Y x ⟨hx, hy⟩;
+  match x with | 0 | 1 => simp_all;
+
+instance : Frame.trivial_nontransitive.IsMonotonic := by
+  constructor;
+  rintro X Y x; match x with | 0 | 1 => simp
+
+instance : Frame.trivial_nontransitive.IsReflexive := by
+  constructor;
+  rintro X x; match x with | 0 | 1 => first | tauto_set | simp_all;
+
+@[simp]
+lemma Frame.trivial_nontransitive.not_transitive : ¬Frame.trivial_nontransitive.IsTransitive := by
+  by_contra hC;
+  have := @(hC.trans Set.univ);
+  have := @this 1 ?_;
+  . have := Set.Subset.antisymm_iff.mp this |>.2;
+    have := @this 0;
+    simp at this;
+  . simp [Frame.box];
+
+@[simp]
+lemma Frame.trivial_nontransitive.not_valid_axiomFour : ¬Frame.trivial_nontransitive ⊧ Axioms.Four (.atom 0) := by
+  apply not_imp_not.mpr isTransitive_of_valid_axiomFour;
+  simp;
+
+end
 
 end Neighborhood
 
@@ -47,23 +94,8 @@ instance : Hilbert.E ⪱ Hilbert.E4 := by
     . simp;
     . apply Sound.not_provable_of_countermodel (𝓜 := FrameClass.E);
       apply not_validOnFrameClass_of_exists_frame;
-      use {
-        World := Fin 2,
-        𝒩 w :=
-          match w with
-          | 0 => ∅
-          | 1 => {{0, 1}},
-      };
-      constructor;
-      . tauto;
-      . apply not_imp_not.mpr isTransitive_of_valid_axiomFour;
-        by_contra hC;
-        have := @(hC.trans {0, 1});
-        have := @this 1 ?_;
-        . have := Set.Subset.antisymm_iff.mp this |>.2;
-          have := @this 0;
-          simp at this;
-        . simp [Frame.box]
+      use Frame.trivial_nontransitive;
+      simp;
 
 end Hilbert
 
