Foundation/Modal/Neighborhood/Logic/EMC4.lean
@@ -42,55 +42,10 @@ instance : Hilbert.EMC ⪱ Hilbert.EMC4 := by
     . simp;
     . apply Sound.not_provable_of_countermodel (𝓜 := FrameClass.EMC);
       apply not_validOnFrameClass_of_exists_frame;
-      use {
-        World := Fin 2,
-        𝒩 w :=
-          match w with
-          | 0 => ∅
-          | 1 => {{0, 1}},
-      };
+      use Frame.trivial_nontransitive;
       constructor;
-      . exact {
-          regular := by
-            rintro X Y x ⟨hx, hy⟩;
-            match x with
-            | 0 => simp_all;
-            | 1 => simp_all;
-          mono := by
-            rintro X Y x;
-            match x with
-            | 0 => simp_all;
-            | 1 => sorry;
-        }
-      . apply not_imp_not.mpr isTransitive_of_valid_axiomFour;
-        by_contra hC;
-        have := @(hC.trans {0, 1});
-        have := @this 1 ?_;
-        . have := Set.Subset.antisymm_iff.mp this |>.2;
-          have := @this 0;
-          simp at this;
-        . simp [Frame.box]
-
-instance : Hilbert.E4 ⪱ Hilbert.EMC4 := by
-  constructor;
-  . apply Hilbert.WithRE.weakerThan_of_subset_axioms;
-    simp;
-  . apply Entailment.not_weakerThan_iff.mpr;
-    use (Axioms.M (.atom 0) (.atom 1));
-    constructor;
-    . simp;
-    . apply Sound.not_provable_of_countermodel (𝓜 := FrameClass.E4);
-      apply not_validOnFrameClass_of_exists_frame;
-      use {
-        World := Fin 2,
-        𝒩 w :=
-          match w with
-          | 0 => ∅
-          | 1 => {{0, 1}},
-      };
-      constructor;
-      . sorry;
-      . sorry;
+      . constructor;
+      . simp;
 
 end Hilbert
 
